coq/Translation/LambdaNRAtoNRAEnv.v
@@ -28,27 +28,94 @@ Section LambdaNRAtoNRAEnv.
 
   Context {fruntime:foreign_runtime}.
 
-  Fixpoint nraenv_of_lnra (op:lnra) : nraenv :=
+  Fixpoint nraenv_of_lambda_nra (op:lambda_nra) : nraenv :=
     match op with
     | LNRAVar x => NRAEnvUnop (ADot x) NRAEnvEnv
     | LNRATable x => NRAEnvGetConstant x
     | LNRAConst d => NRAEnvConst d
-    | LNRABinop b op1 op2 => NRAEnvBinop b (nraenv_of_lnra op1) (nraenv_of_lnra op2)
-    | LNRAUnop u op1 => NRAEnvUnop u (nraenv_of_lnra op1)
-    | LNRAMap lop1 op2 => NRAEnvMap (nraenv_of_lnra_lambda lop1) (nraenv_of_lnra op2)
-    | LNRAMapConcat lop1 op2 => NRAEnvMapConcat (nraenv_of_lnra_lambda lop1) (nraenv_of_lnra op2)
-    | LNRAProduct op1 op2 => NRAEnvProduct (nraenv_of_lnra op1) (nraenv_of_lnra op2)
-    | LNRAFilter lop1 op2 => NRAEnvSelect (nraenv_of_lnra_lambda lop1) (nraenv_of_lnra op2)
+    | LNRABinop b op1 op2 => NRAEnvBinop b (nraenv_of_lambda_nra op1) (nraenv_of_lambda_nra op2)
+    | LNRAUnop u op1 => NRAEnvUnop u (nraenv_of_lambda_nra op1)
+    | LNRAMap lop1 op2 => NRAEnvMap (nraenv_of_lnra_lambda lop1) (nraenv_of_lambda_nra op2)
+    | LNRAMapConcat lop1 op2 => NRAEnvMapConcat (nraenv_of_lnra_lambda lop1) (nraenv_of_lambda_nra op2)
+    | LNRAProduct op1 op2 => NRAEnvProduct (nraenv_of_lambda_nra op1) (nraenv_of_lambda_nra op2)
+    | LNRAFilter lop1 op2 => NRAEnvSelect (nraenv_of_lnra_lambda lop1) (nraenv_of_lambda_nra op2)
     end
   with nraenv_of_lnra_lambda (lop:lnra_lambda) : nraenv :=
     match lop with
     | LNRALambda x op =>
-      NRAEnvAppEnv (nraenv_of_lnra op) (NRAEnvBinop AConcat NRAEnvEnv (NRAEnvUnop (ARec x) NRAEnvID))
+      NRAEnvAppEnv (nraenv_of_lambda_nra op) (NRAEnvBinop AConcat NRAEnvEnv (NRAEnvUnop (ARec x) NRAEnvID))
     end.
 
   Context (h:brand_relation_t).
-  Context (global_env:list (string*data)).
-    
+  Context (global_env:bindings).
+
+  Lemma nraenv_of_lambda_nra_never_uses_id :
+    forall env:bindings, forall q:lambda_nra, forall d1 d2:data,
+          nraenv_eval h global_env
+                      (nraenv_of_lambda_nra q) (drec env) d1 =
+          nraenv_eval h global_env
+                      (nraenv_of_lambda_nra q) (drec env) d2.
+  Proof.
+    lambda_nra_cases (induction q) Case
+    ; intros; unfold nraenv_eval in *; simpl in *
+    ; autorewrite with lambda_nra; try reflexivity.
+    - Case "LNRABinop"%string.
+      rewrite (IHq1 d1 d2).
+      rewrite (IHq2 d1 d2).
+      reflexivity.
+    - Case "LNRAUnop"%string.
+      rewrite (IHq d1 d2).
+      reflexivity.
+    - Case "LNRAMap"%string.
+      rewrite (IHq2 d1 d2).
+      reflexivity.
+    - Case "LNRAMapConcat"%string.
+      rewrite (IHq2 d1 d2).
+      reflexivity.
+    - Case "LNRAProduct"%string.
+      rewrite (IHq1 d1 d2).
+      rewrite (IHq2 d1 d2).
+      reflexivity.
+    - Case "LNRAFilter"%string.
+      rewrite (IHq2 d1 d2).
+      reflexivity.
+  Qed.
+
+  Theorem nraenv_of_lambda_nra_correct :
+    forall q:lambda_nra, forall env:bindings, forall d:data,
+      lambda_nra_eval h global_env env q =
+      nraenv_eval h global_env
+                  (nraenv_of_lambda_nra q) (drec env) d.
+  Proof.
+    lambda_nra_cases (induction q) Case
+    ; intros; unfold nraenv_eval in *; simpl in *
+    ; autorewrite with lambda_nra; try reflexivity.
+    - Case "LNRABinop"%string.
+      rewrite (IHq1 _ d).
+      rewrite (IHq2 _ d).
+      reflexivity.
+    - Case "LNRAUnop"%string.
+      rewrite (IHq _ d).
+      reflexivity.
+    - Case "LNRAMap"%string.
+      rewrite <- (IHq2 _ d).
+      simpl.
+      apply olift_ext; intros.
+      apply lift_oncoll_ext; intros.
+      subst.
+      f_equal.
+      apply rmap_ext; intros.
+      autorewrite with lambda_nra.
+      rewrite (IHq1 _ x).
+      admit.
+    - Case "LNRAMapConcat"%string.
+      admit.
+    - Case "LNRAProduct"%string.
+      admit.
+    - Case "LNRAFilter"%string.
+      admit.
+  Admitted.
+  
   Theorem nraenv_of_lnra_lambda_correct :
     forall env:bindings, forall lop:lnra_lambda, forall d:data,
       lnra_lambda_eval h global_env env lop d =
@@ -57,9 +124,9 @@ Section LambdaNRAtoNRAEnv.
   Proof.
     destruct lop.
     revert env s.
-    lnra_cases (induction l) Case
+    lambda_nra_cases (induction l) Case
     ; intros; unfold nraenv_eval in *; simpl in *
-    ; autorewrite with lnra.
+    ; autorewrite with lambda_nra.
     - Case "LNRAVar"%string.
       unfold edot, rec_concat_sort.
       rewrite assoc_lookupr_drec_sort.
@@ -113,10 +180,10 @@ Section LambdaNRAtoNRAEnv.
   Definition eval_nraenv_q (Qe:nraenv) (input:data) : option data :=
     nraenv_eval h global_env Qe (drec nil) input.
 
-  Theorem eval_nraenv_q_correct (Q:lnra -> lnra) (input:data) :
-    eval_q h global_env Q input = eval_nraenv_q (nraenv_of_lnra_lambda (q_to_lambda Q)) input.
+  Theorem eval_nraenv_q_correct (Q:lambda_nra -> lambda_nra) (input:data) :
+    eval_lnra_lambda h global_env Q input = eval_nraenv_q (nraenv_of_lnra_lambda (q_to_lambda Q)) input.
   Proof.
-    unfold eval_q, eval_nraenv_q.
+    unfold eval_lnra_lambda, eval_nraenv_q.
     rewrite nraenv_of_lnra_lambda_correct.
     reflexivity.
   Qed.
